sketch listsum_compiled_correctly and connection from Gallina to RISCV machine

src/ListSumExample.v
@@ -18,48 +18,53 @@ Require Import compiler.NameGen.
 
 Require Import riscv.RiscvBitWidths32.
 
+Local Notation RiscvMachine := (@RiscvMachine RiscvBitWidths32 (mem wXLEN) state).
+
 
 Module ExampleSrc.
 
-Import ExprImpNotations. (* only inside this module *)
+  Import ExprImpNotations. (* only inside this module *)
   
-Definition n: var := 1.
-Definition i: var := 2.
-Definition sumreg: var := 3.
-Definition a: var := 4.
+  Definition n: var := 1.
+  Definition i: var := 2.
+  Definition sumreg: var := 3.
+  Definition a: var := 4.
 
 
-Definition input_base: Z := 512.
+  Definition input_base: Z := 512.
 
-(* Inputs:
+  (* Inputs:
      n: length of list, at address input_base
      A: list of 32-bit ints of length n, at address input_base + 4
    Output: in register 'sumreg'
-*)
+   *)
 
-Example listsum: stmt :=
-  sumreg <-- 0;
-  n <-* input_base;
-  i <-- 0;
-  while i < n do
-    a <-* (input_base + 4)%Z + 4 * i;
-    sumreg <-- sumreg + a;
-    i <-- i + 1
-  done.
+  Example listsum: stmt :=
+    sumreg <-- 0;
+    n <-* input_base;
+    i <-- 0;
+    while i < n do
+      a <-* (input_base + 4)%Z + 4 * i;
+      sumreg <-- sumreg + a;
+      i <-- i + 1
+    done.
+
+  Print listsum.
 
 End ExampleSrc.
 
-(* Here we compile: exprImp2Riscv is the main compilation function *)
-Definition listsum_riscv: list Instruction := Eval cbv in exprImp2Riscv ExampleSrc.listsum.
+Print ExampleSrc.listsum.
 
-Print listsum_riscv.
+(* Here we compile: exprImp2Riscv is the main compilation function *)
+Definition listsum_riscv: list Instruction := exprImp2Riscv ExampleSrc.listsum.
+
+Eval cbv in listsum_riscv.
 
 Eval simpl in (List.length listsum_riscv).
 
-Definition listsum_bits: list (word 32) :=
-  Eval cbv in (map (fun i => ZToWord 32 (encode i)) listsum_riscv).
+Definition listsum_bits: list (word 32) := (map (fun i => ZToWord 32 (encode i)) listsum_riscv).
 
-Print listsum_bits.
+Eval cbv in listsum_bits.
 
 Definition mk_input(l: list nat): list (word 32) :=
   (natToWord 32 (List.length l)) :: (List.map (natToWord 32) l).
@@ -74,7 +79,7 @@ Definition initialMem_without_instructions(l: list nat): list (word 32) :=
 
 Definition instructionMemStart: nat := 0.
 
-Definition initialRiscvMachineCore: RiscvMachineCore := {|
+Definition initialRiscvMachineCore: @RiscvMachineCore _ state := {|
   registers := initialRegs;
   pc := $instructionMemStart;
   nextPC := $instructionMemStart ^+ $4;
@@ -103,6 +108,89 @@ Definition listsum_final(fuel: nat)(l: list nat): RiscvMachine :=
   snd (run fuel (initialRiscvMachine l)).
 
 Definition listsum_res(fuel: nat)(l: list nat): word wXLEN :=
-  (listsum_final fuel l).(core).(registers) ExampleSrc.sumreg.
+  getReg (listsum_final fuel l).(core).(registers) ExampleSrc.sumreg.
 
 Eval vm_compute in (listsum_res 400 [4; 5; 3]).
+
+
+Definition initialMemH(l: list nat): Memory.mem :=
+  fun (a: word 32) => if dec (wordToZ a < ExampleSrc.input_base)%Z then
+                        None (* make inaccessible to protect instruction memory *)
+                      else
+                        nth_error (mk_input l) ((wordToNat a - Z.to_nat ExampleSrc.input_base)  / 4).
+
+Definition evalH(fuel: nat)(l: list nat): option (state * Memory.mem) :=
+  eval_stmt fuel empty (initialMemH l) ExampleSrc.listsum.
+
+Definition listsum_res_H(fuel: nat)(l: list nat): option (word 32) :=
+  match evalH fuel l with
+  | Some (regs, m) => get regs ExampleSrc.sumreg
+  | _ => None
+  end.
+
+Eval vm_compute in (listsum_res_H 40 [3; 7; 6]).
+
+
+Lemma listsum_compiled_correctly: forall l fuelH res,
+(*    Z.to_nat ExampleSrc.input_base + 4 + 4 * length l <= pow2 32 ->*)
+    listsum_res_H fuelH l = Some res ->
+    exists fuelL, listsum_res fuelL l = res.
+Proof.
+  intros.
+  unfold listsum_res_H, evalH in H. destruct_one_match_hyp; try discriminate.
+  destruct p as [finalRegsH finalMemH].
+  unfold listsum_res, listsum_final.
+  pose proof exprImp2Riscv_correct as Q.
+  specialize Q with (sH := ExampleSrc.listsum) (initialL := (initialRiscvMachine_without_instructions l)).
+  unfold Pipeline.evalH in Q.
+  edestruct Q as [fuelL P]; try eassumption.
+  - change 14 with (5 + 9). rewrite Nat.pow_add_r.
+    pose proof (zero_lt_pow2 9).
+    forget (pow2 9) as x.
+    apply lt_mul_mono; cbv; omega.
+  - reflexivity.
+  - match goal with
+    | |- context [length ?x] => let r := eval cbv in (length x) in change (length x) with r
+    end.
+    unfold initialRiscvMachine_without_instructions, putProgram.
+    cbv [machineMem with_pc with_nextPC with_machineMem].
+    pose proof store_word_list_preserves_memSize as R.
+    unfold wXLEN, bitwidth, RiscvBitWidths.bitwidth, RiscvBitWidths32 in R|-*; rewrite R.
+    clear R.
+    unfold zero_mem.
+    unfold Memory.memSize, mem_is_Memory.
+    rewrite const_mem_mem_size.
+    + apply Nat.le_trans with (m := Z.to_nat ExampleSrc.input_base).
+      * cbv. omega.
+      * omega.
+    + (* TODO make sure mem size is a multiple of 8 *) admit.
+    + admit. (* todo bounds *)
+  - cbv [length].
+    unfold initialMemH, FlatToRiscv.mem_inaccessible.
+    intros. unfold Memory.read_mem in *.
+    do 2 (destruct_one_match_hyp; try discriminate).
+    unfold FlatToRiscv.not_in_range.
+    right.
+    (* TODO prevent underflow of substraction *)
+    admit.
+  - exists fuelL. apply P. apply H.
+Admitted.    
+
+
+Definition sum_gallina(l: list nat): nat := List.fold_right plus 0 l.
+
+Lemma hl_listsum_correct: forall l,
+    exists fuel, listsum_res_H fuel l = Some (natToWord 32 (sum_gallina l)).
+Proof.
+  (* Future work: Proof framework to connect ExprImp programs with Gallina programs *)
+Admitted.
+
+
+Lemma listsum_will_run_correctly: forall l,
+    (* TODO: bound on length of l *)
+    exists fuelL, listsum_res fuelL l = $(sum_gallina l).
+Proof.
+  intros.
+  destruct (hl_listsum_correct l) as [fuelH E].
+  apply (listsum_compiled_correctly l fuelH _ E).
+Qed.
